Classes/Galois.v
@@ -5,19 +5,19 @@ Require Import PreorderedSet.
 
 Class Galois (A A' : Type) `{A'_preorder: PreorderedSet A'} : Type :=
 {
-  gamma : A' -> A -> Prop;
-  gamma_monotone : monotone gamma;
+  γ : A' -> ℘ A;
+  gamma_monotone : monotone γ;
 }.
-Arguments gamma : simpl never.
-Hint Extern 10 (gamma _ _) => constructor : soundness.
+Arguments γ : simpl never.
+Hint Extern 10 (γ _ _) => constructor : soundness.
 
 Ltac gamma_destruct := repeat
   match goal with
-  | x : gamma _  _ |- _ => inv x
+  | x : γ _  _ |- _ => inv x
   end.
 
 Lemma gamma_preorder {A A'} `{A_galois : Galois A A'}: forall (a' a2' : A') (a : A), 
-    preorder a' a2' -> gamma a' a -> gamma a2' a.
+    preorder a' a2' -> γ a' a -> γ a2' a.
 Proof.
   intros a a' b Hpre Hgamma.
   pose proof gamma_monotone as Hmono.
@@ -27,7 +27,7 @@ Qed.
 
 Lemma gamma_join_left {A A'} `{A'_joinable : Joinable A'} 
   `{A_galois : @Galois A A' T_preorder} : ∀ (a : A) (a'1 a'2 : A'),
-  gamma a'1 a → gamma (join_op a'1 a'2) a.
+  γ a'1 a → γ (join_op a'1 a'2) a.
 Proof. 
   intros. apply (gamma_preorder a'1). 
   apply join_upper_bound_left. assumption.
@@ -35,7 +35,7 @@ Qed.
 
 Lemma gamma_join_right {A A'} `{A'_joinable : Joinable A'} 
   `{A_galois : @Galois A A' T_preorder} : ∀ (a : A) (a'1 a'2 : A'),
-  gamma a'2 a → gamma (join_op a'1 a'2) a.
+  γ a'2 a → γ (join_op a'1 a'2) a.
 Proof. 
   intros. apply (gamma_preorder a'2). 
   apply join_upper_bound_right. assumption.
@@ -43,6 +43,6 @@ Qed.
 
 Ltac apply_widen :=
   match goal with
-  | H : preorder ?a ?b, I : gamma ?a ?c |- gamma ?b ?c =>
+  | H : preorder ?a ?b, I : γ ?a ?c |- γ ?b ?c =>
       eapply gamma_preorder; apply H + apply I
   end.
